

1. **with replacement**

$\Omega = \{RR, RG, RB, GG, GR, GB, BB, BG, BR\}$

probability of any individual outcome = $1/9$

without replacement

$\Omega = \{RG, RB, GR, GB, BR, BG\}$

probability of any individual outcome = $1/6$

2. E = the event that the sum of the dice is odd

F = at least one of the dice lands on 1

G = the sum of the dice is 5

How many elementary outcomes are there in the events

E intersect F ? 6

E union F ? 23

F intersect G ? 2

$E \setminus F$ (E without F)? 12

E intersect F intersect G ? 2

ok so the entire S is

$S = \{$
 $(1,1), (1,2), (1,3), (1,4), (1,5), (1,6),$
 $(2,1), (2,2), (2,3), (2,4), (2,5), (2,6),$
 $(3,1), (3,2), (3,3), (3,4), (3,5), (3,6),$
 $(4,1), (4,2), (4,3), (4,4), (4,5), (4,6),$
 $(5,1), (5,2), (5,3), (5,4), (5,5), (5,6),$
 $(6,1), (6,2), (6,3), (6,4), (6,5), (6,6)$
 $\}$

The events that the sum of the dice is odd are

$E_events = \{$
 ~~$(1,1), (1,2), (1,3), (1,4), (1,5), (1,6),$~~
 ~~$(2,1), (2,2), (2,3), (2,4), (2,5), (2,6),$~~
 ~~$(3,1), (3,2), (3,3), (3,4), (3,5), (3,6),$~~
 ~~$(4,1), (4,2), (4,3), (4,4), (4,5), (4,6),$~~
 ~~$(5,1), (5,2), (5,3), (5,4), (5,5), (5,6),$~~
 ~~$(6,1), (6,2), (6,3), (6,4), (6,5), (6,6)$~~
 $\}$
 $= \{$
 $(1,2), (1,4), (1,6),$
 $(2,1), (2,3), (2,5),$
 $(3,2), (3,4), (3,6),$
 $(4,1), (4,3), (4,5),$
 $(5,2), (5,4), (5,6),$
 $(6,1), (6,3), (6,5)$
 $\}$

}

F events = {
 (1,1),(1,2),(1,3),(1,4),(1,5),(1,6),
 (2,1),(3,1),(4,1),(5,1),(6,1)
}

G events = {
 (1,4),(2,3),(3,2),(4,1)
}

Then E intersect F has events

{
 (1,2),(1,4),(1,6)
 (2,1),(4,1),(6,1)
}

Then E union F has events

{
 (1,1),(1,2),(1,3),(1,4),(1,5),(1,6),
 (2,1),(2,3),(2,5),
 (3,1),(3,2),(3,4),(3,6),
 (4,1),(4,3),(4,5),
 (5,1),(5,2),(5,4),(5,6),
 (6,1),(6,3),(6,5)
}

F intersect G has events

{
 (1,4),(4,1)
}

E without F has events

{
 (2,3),(2,5),
 (3,2),(3,4),(3,6),
 (4,3),(4,5),
 (5,2),(5,4),(5,6),
 (6,3),(6,5)
}

E intersect F intersect G has events

{
 (1,4),(4,1)
}

3. n socks. 3 are red.

if $P(X=2) = .5$.

That is to say that if we chose 2 socks from the n group of socks, the probability both socks chosen are red is .5.

What's the value of n ?

$$n = 3 + y$$

y = the number of non red socks

We can get the number of combinations with n choose $r = n! / (n-r)!r!$

$$= n! / (n-2)!2! = n(n-1)/2$$

we know that half of those permutations must yield 2 red socks since $P(X=2) = .5$

How is $P(X=2)$ determined?

$$P(X=2) = \# \text{ of ways you can get two red socks} / \# \text{ of ways you can get two socks}$$

we know the denominator. The number of ways we can get two socks is $n(n-1) / 2$

so setting up an initial equation we have $.5 = \# \text{ of ways we can get two red socks} / n(n-1)/2$

we know there is 3 red socks. Lets call them R_1, R_2 and R_3 .

Then the distinct combinations we can make of those 3 socks are $(R_1, R_2), (R_1, R_3)$ and (R_2, R_3)

Alternatively we can say 3 choose 2 and we get $3(2) / 2 = 3$

so now we have $P(X=2) = .5$ and $P(X=2) = 3 / [n(n-1)/2] = 6/(n(n-1))$

Solving $.5 = 6/[n(n-1)]$ gives us **$n=4$** .

4.

We have from (c) $A_1, A_2, \dots, A_n \in \mathcal{F}$ then $\bigcup_{i=1}^n A_i \in \mathcal{F}$

We have from (b) that if $A_i \in \mathcal{F}$ then $\Omega \setminus A_i \in \mathcal{F}$

another way to write (b) is if $A_i \in \mathcal{F}$ then $A_i^c \in \mathcal{F}$

Using both (b) and (c) we have that $\bigcup_{i=1}^n A_i^c \in \mathcal{F}$

Using (b) we then have $\left(\bigcup_{i=1}^n A_i^c\right)^c \in \mathcal{F}$

By De Morgan's Law we have $\left(\bigcup_{i=1}^n A_i^c\right)^c = \left(\bigcap_{i=1}^n (A_i^c)^c\right) \in \mathcal{F}$

$$(A_i^c)^c = A_i$$

So we have $\bigcap_{i=1}^n A_i \in \mathcal{F}$

N.B. I initially attempted this by showing that $A_1 \cap A_2 \cap \dots \cap A_n \in \mathcal{F}$.
I had ran into some road blocks but I think I figured it out. Here's is that proof as well.

We have from (c) $A_1, A_2, \dots, A_n \in \mathcal{F}$ then $\bigcup_{i=1}^n A_i \in \mathcal{F}$

we need to prove that

$$P(A_1 \cup A_2 \cup \dots \cup A_n) = \sum_{i=1}^n P(A_i) - \sum_{i \leq j \leq n} P(A_i \cap A_j) + \sum_{i \leq j \leq l \leq n} P(A_i \cap A_j \cap A_l) + \dots \pm P(A_1 \cap A_2 \cap \dots \cap A_n)$$

since that will show that $(A_1 \cap A_2 \cap \dots \cap A_n) \in \bigcup_{i=1}^n A_i \in \mathcal{F}$

Proof:

n=2 case

$$A \cup B = (A \setminus B) \cup (A \cap B) \cup (B \setminus A) \text{ (disjoint union)}$$

$$P(A \cup B) = P(A \setminus B) + P(A \cap B) + P(B \setminus A)$$

add and subtract $P(A \cap B)$

$$P(A \cup B) = P(A \setminus B) + P(A \cap B) + P(B \setminus A) + P(A \cap B) - P(A \cap B)$$

we also have that $P(A \setminus B) + P(A \cap B) = P(A)$ and $P(B \setminus A) + P(A \cap B) = P(B)$

substituting this in we get

$$P(A \cup B) = P(A) + P(B) - P(A \cap B)$$

this can be rewritten to

$$P(A_1 \cup A_2) = P(A_1) + P(A_2) - P(A_1 \cap A_2) = \sum_{i=1}^{n=2} P(A_i) - \sum_{i \leq j \leq n} P(A_i \cap A_j)$$

n=3 case

$$P(A_1 \cup A_2 \cup A_3) = P(A_1 \setminus (A_2 \cup A_3)) + P(A_1 \cap (A_2 \cup A_3)) + P((A_2 \cup A_3) \setminus A_1)$$

we have the following:

$$P(A_1 \setminus (A_2 \cup A_3)) = P(A_1 \setminus A_2) - P(A_1 \cap A_3) + P(A_1 \cap A_2 \cap A_3)$$

$$P(A_1 \cap (A_2 \cup A_3)) = P(A_1 \cap A_2) + P(A_1 \cap A_3) - P(A_1 \cap A_2 \cap A_3)$$

$$P((A_2 \cup A_3) \setminus A_1) = P(A_2 \setminus A_1) + P(A_3 \setminus A_1) - P(A_2 \cap A_3) + P(A_1 \cap A_2 \cap A_3)$$

$$\Rightarrow P(A_1 \cup A_2 \cup A_3) = P(A_1 \setminus A_2) - P(A_1 \cap A_3) + P(A_1 \cap A_2 \cap A_3) + P(A_1 \cap A_2) + P(A_1 \cap A_3) - P(A_1 \cap A_2 \cap A_3) + P(A_2 \setminus A_1) + P(A_3 \setminus A_1) - P(A_2 \cap A_3) + P(A_1 \cap A_2 \cap A_3)$$

we also have:

$$P(A_1) = P(A_1 \setminus A_2) + P(A_1 \cap A_2) = P(A_1 \setminus A_3) + P(A_1 \cap A_3)$$

$$P(A_2) = P(A_2 \setminus A_1) + P(A_2 \cap A_1) = P(A_2 \setminus A_3) + P(A_2 \cap A_3)$$

$$P(A_3) = P(A_3 \setminus A_2) + P(A_3 \cap A_2) = P(A_3 \setminus A_1) + P(A_3 \cap A_1)$$

$$\Rightarrow P(A_1 \cup A_2 \cup A_3) = P(A_1) + P(A_3) + P(A_2 \setminus A_1) - P(A_1 \cap A_3) - P(A_2 \cap A_3) + P(A_1 \cap A_2 \cap A_3)$$

add and subtract $P(A_2 \cap A_1)$ to the right hand side

$$\Rightarrow P(A_1 \cup A_2 \cup A_3) = P(A_1) + P(A_2) + P(A_3) - P(A_2 \cap A_1) - P(A_1 \cap A_3) - P(A_2 \cap A_3) + P(A_1 \cap A_2 \cap A_3) = \sum_{i=1}^{n=3} P(A_i) - \sum_{i \leq j \leq n} P(A_i \cap A_j) + \sum_{i \leq j \leq l \leq n} P(A_i \cap A_j \cap A_l)$$

n=n case

let

$$P(A_1 \cup A_2 \cup \dots \cup A_n) = \sum_{i=1}^n P(A_i) - \sum_{i \leq j \leq n} P(A_i \cap A_j) + \sum_{i \leq j \leq l \leq n} P(A_i \cap A_j \cap A_l) + \dots \pm P(A_1 \cap A_2 \cap \dots \cap A_n)$$

be true

then prove that

$$P(A_1 \cup A_2 \cup \dots \cup A_{n+1}) = \sum_{i=1}^{n+1} P(A_i) - \sum_{i \leq j \leq n+1} P(A_i \cap A_j) + \sum_{i \leq j \leq l \leq n+1} P(A_i \cap A_j \cap A_l) + \dots \pm P(A_1 \cap A_2 \cap \dots \cap A_{n+1})$$

$$P(A_1 \cup A_2 \cup \dots \cup A_{n+1}) = P\{(A_1 \cup A_2 \cup \dots \cup A_n) \cup A_{n+1}\}$$

we can use the n=2 case on this second part

$$P\{(A_1 \cup A_2 \cup \dots \cup A_n) \cup A_{n+1}\} = P(A_1 \cup A_2 \cup \dots \cup A_n) + P(A_{n+1}) - P\{(A_1 \cup A_2 \cup \dots \cup A_n) \cap A_{n+1}\}$$

$$P\{(A_1 \cup A_2 \cup \dots \cup A_n) \cap A_{n+1}\} = P\{(A_1 \cap A_{n+1}) \cup (A_2 \cap A_{n+1}) \cup \dots \cup (A_n \cap A_{n+1})\}$$

so we have

$$P(A_1 \cup A_2 \cup \dots \cup A_{n+1}) = P(A_1 \cup A_2 \cup \dots \cup A_n) + P(A_{n+1}) - P\{(A_1 \cap A_{n+1}) \cup (A_2 \cap A_{n+1}) \cup \dots \cup (A_n \cap A_{n+1})\}$$

The first and third term we can use the formula on so we get.

$$\begin{aligned} &= \sum_{i=1}^n P(A_i) - \sum_{i \leq j \leq n} P(A_i \cap A_j) + \sum_{i \leq j \leq l \leq n} P(A_i \cap A_j \cap A_l) + \dots \pm P(A_1 \cap A_2 \cap \dots \cap A_n) \\ &\quad + P(A_{n+1}) \\ &\quad - \sum_{i=1}^n P(A_i \cap A_{n+1}) + \sum_{i \leq j \leq n} P(A_i \cap A_{n+1} \cap A_j) - \sum_{i \leq j \leq l \leq n} P(A_i \cap A_{n+1} \cap A_j \cap A_l) + \dots \pm P(A_1 \cap A_2 \cap \dots \cap A_n \cap A_{n+1}) \end{aligned}$$

$$\text{Notice how } \sum_{i=1}^n P(A_i) + P(A_{n+1}) = \sum_{i=1}^{n+1} P(A_i)$$

$$\text{and how } - \sum_{i \leq j \leq n} P(A_i \cap A_j) - \sum_{i=1}^n P(A_i \cap A_{n+1}) = - \sum_{i \leq j \leq n+1} P(A_i \cap A_j)$$

and the rest of the terms combine as well

which gives us

$$P(A_1 \cup A_2 \cup \dots \cup A_{n+1}) = \sum_{i=1}^{n+1} P(A_i) - \sum_{i \leq j \leq n+1} P(A_i \cap A_j) + \sum_{i \leq j \leq l \leq n+1} P(A_i \cap A_j \cap A_l) + \dots \pm P(A_1 \cap A_2 \cap \dots \cap A_{n+1})$$

